iris/ProofKexecB3.v
@@ -1092,7 +1092,7 @@ Section KexecB3Body.
                            Hivalid & Hload & #Hity & Hfrz & Hkeep & Hru)".
     iDestruct (kxc_load_peel with "Hload") as
       (datl) "(%Hiok & %Hdok & %Hddix & %Hdoc & %Hduq & Hdlk & Hdiat & Hmeta & Hmap
-               & Hblocks & Hdview)".
+               & Hblocks & Hdview & Hfview)".
     pose proof Hiok as Hiok'.
     destruct Hiok' as (Hbmwf & Hbmcov & Hdaddr & Hdty & Hszb & Hholes & Hsized).
     iDestruct (proc_priv_bare_acc gf (proc_addr jp) pidv V with "Hpriv")
@@ -1129,7 +1129,7 @@ Section KexecB3Body.
     iDestruct ("Hpvbk" with "Hppid") as "Hpriv".
     iDestruct (kxc_load_seal gfs gi cov logstart kf inumf dnf bmf datl
                  Hiok Hdok Hddix Hdoc Hduq
-                 with "Hdlk Hdiat Hmeta Hmap Hblocks Hdview") as "Hload".
+                 with "Hdlk Hdiat Hmeta Hmap Hblocks Hdview Hfview") as "Hload".
     iDestruct (A.kxa_bs3_join with "Hbs1 Hbs2") as "Hbs".
     iDestruct (kxc_open_intro gfs gi cn cov logstart dev pidv kf qf sf gyf
                  inumf dnf bmf gilf gislf
