iris/ProofNamex.v
@@ -3148,7 +3148,7 @@ Section ProofNamexMain.
                                       & Y23 & Y24 & Y25 & Ythr).
                    iDestruct "Hload" as (datl)
                      "(%Hiok & %Hdok & %Hddix & %Hdoc & %Hduq & Hdlnk & Hdiat & Hmeta & Haddrs & Hind &
-                       Hblocks & Hdview)".
+                       Hblocks & Hdview & Hfview)".
                    iDestruct "Hmeta" as "(Hity & Himaj & Himin & Hinl & Hisz)".
                    iEval (rewrite /i_type) in "Hity".
                    (* +0xc6 lh a5,68(s4) : ip->type *)
@@ -3276,7 +3276,7 @@ Section ProofNamexMain.
                      iPoseProof (nxi_080 with "Htext") as "Hj5a".
                      iAssert (ic_loaded gfs gi cov logstart ik iinum dnl bml)
                        with "[Hdiat Hity Himaj Himin Hinl Hisz Haddrs Hind
-                              Hblocks Hdlnk Hdview]" as "Hload".
+                              Hblocks Hdlnk Hdview Hfview]" as "Hload".
                      { rewrite /ic_loaded. iExists datl.
                        iSplitR; [iPureIntro; exact Hiok |].
                        iSplitR; [iPureIntro; exact Hdok |].
@@ -3617,7 +3617,7 @@ Section ProofNamexMain.
                                      ltac:(vm_compute; reflexivity) HP2regs).
                        iAssert (ic_loaded gfs gi cov logstart ik iinum dnl bml)
                          with "[Hdiat Hity Himaj Himin Hinl Hisz Haddrs Hind
-                                Hblocks Hdlnk Hdview]" as "Hload".
+                                Hblocks Hdlnk Hdview Hfview]" as "Hload".
                        { rewrite /ic_loaded. iExists datl.
                          iSplitR; [iPureIntro; exact Hiok |].
                          iSplitR; [iPureIntro; exact Hdok |].
@@ -3813,7 +3813,7 @@ Section ProofNamexMain.
                                 Hcwdr Hname Hbs1 Hbs2 Hlog Hkeep Hru Hslkd
                                 Hdep Hidev Hiinum Hivalid Hfrz Hdiat Hity
                                 Himaj Himin Hinl Hisz Haddrs Hind Hblocks
-                               Hdlnk Hdview]"
+                               Hdlnk Hdview Hfview]"
                          as "Hdlblk".
                        { iIntros (CIDz Hsz Mz) "%Hregz Hcg Hcnt Hextc Hclmc Hpc Hpath".
                          pose proof Hregz as Hrz.
@@ -4006,7 +4006,7 @@ Section ProofNamexMain.
                          iDestruct "Hmap" as "[Haddrs Hind]".
                          iAssert (ic_loaded gfs gi cov logstart ik iinum dnl
                                     bml)
-                           with "[Hdiat Hmeta Haddrs Hind Hblocks Hdlnk Hdview]"
+                           with "[Hdiat Hmeta Haddrs Hind Hblocks Hdlnk Hdview Hfview]"
                            as "Hload".
                          { rewrite /ic_loaded. iExists datl.
                            iSplitR; [iPureIntro; exact Hiok |].
@@ -4015,7 +4015,7 @@ Section ProofNamexMain.
                            iSplitR; [iPureIntro; exact Hdoc |].
                            iSplitR; [iPureIntro; exact Hduq |].
                            iSplitL "Hdlnk"; [iExact "Hdlnk" |].
-                           iFrame "Hdiat Hmeta Haddrs Hind Hblocks Hdview". }
+                           iFrame "Hdiat Hmeta Haddrs Hind Hblocks Hdview Hfview". }
                          iDestruct (nx_bs3_join with "Hbs1 Hbs2") as "Hbslot".
                          destruct found.
                          - (* ============ FOUND: recurse on the child ==== *)
@@ -4618,7 +4618,7 @@ Section ProofNamexMain.
                      iPoseProof (nxi_05a with "Htext") as "Hj5a".
                      iAssert (ic_loaded gfs gi cov logstart ik iinum dnl bml)
                        with "[Hdiat Hity Himaj Himin Hinl Hisz Haddrs Hind
-                              Hblocks Hdlnk Hdview]" as "Hload".
+                              Hblocks Hdlnk Hdview Hfview]" as "Hload".
                      { rewrite /ic_loaded. iExists datl.
                        iSplitR; [iPureIntro; exact Hiok |].
                        iSplitR; [iPureIntro; exact Hdok |].
